src/tls/Format.UncompressedPointRepresentation.fsti
@@ -1,0 +1,41 @@
+module Format.UncompressedPointRepresentation
+
+module B = FStar.Bytes
+module U32 = FStar.UInt32
+module LP = LowParse.SLow
+
+(* Types *)
+
+(*
+    https://tlswg.github.io/tls13-spec/draft-ietf-tls-tls13.html#rfc.section.4.2.8.2
+
+    struct {
+        uint8 legacy_form = 4;
+        opaque X[coordinate_length];
+        opaque Y[coordinate_length];
+    } UncompressedPointRepresentation;
+*)
+
+type lbytes32 n = B.lbytes (UInt32.v n)
+
+type uncompressedPointRepresentation (coordinate_length:U32.t) = {
+    legacy_form : l:B.byte{l = 4uy};
+    x           : lbytes32 coordinate_length;
+    y           : lbytes32 coordinate_length
+}
+
+val uncompressedPointRepresentation_parser_kind (coordinate_length:U32.t): LP.parser_kind
+
+val uncompressedPointRepresentation_parser (coordinate_length:U32.t)
+  : LP.parser (uncompressedPointRepresentation_parser_kind coordinate_length) (uncompressedPointRepresentation coordinate_length) 
+
+inline_for_extraction
+val uncompressedPointRepresentation_parser32 (coordinate_length:U32.t) 
+  : LP.parser32 (uncompressedPointRepresentation_parser coordinate_length)
+
+val uncompressedPointRepresentation_serializer (coordinate_length:U32.t) 
+  : LP.serializer (uncompressedPointRepresentation_parser coordinate_length)
+
+inline_for_extraction
+val uncompressedPointRepresentation_serializer32 (coordinate_length:U32.t) 
+  : LP.serializer32 (uncompressedPointRepresentation_serializer coordinate_length)
